Added final string predicates

project2/strings2.dfy
@@ -1,3 +1,14 @@
+/* 
+	CS4504 - Formal Verification
+	Dr Vasileios Koutavas
+	Group Assignment 2 - Predicates about string search
+	Stefano Lupo:		14334933 - 4 hours 
+		It really should have only taken 1 hour 
+		Most of the time was spent trying to figure out why certain approaches would fail in Dafny
+	Rowan Sutton:		13330793 - 3 Hours
+		About 2 of the 3 hours were spent debugging the substring and k substring premises
+*/
+
 predicate isPrefixPred(pre:string, str:string)
 {
 	(|pre| <= |str|) && pre == str[..|pre|]
@@ -5,123 +16,42 @@ predicate isPrefixPred(pre:string, str:string)
 
 predicate isNotPrefixPred(pre:string, str:string)
 {
-	// TODO: your formula should not contain &&
-	|pre| > |str| || !(forall x :: 0 <= x < |pre| ==> pre[x] == str[x])
-
-	// Not sure why these don't work..
-	//|pre| > |str| || (exists x :: 0 <= x < |pre| ==> pre[x] != str[x])
+	|pre| > |str| || !(pre == str[..|pre|])  // DeMorgan
 }
-
-/*
-lemma PrefixNegationLemmaExpanded(pre:string, str:string) 
-ensures isPrefixPred(pre, str) ==> !(isNotPrefixPred(pre, str))
-ensures !(isNotPrefixPred(pre, str)) ==> isPrefixPred(pre, str)
-ensures !(isPrefixPred(pre, str)) ==> isNotPrefixPred(pre, str)
-ensures isNotPrefixPred(pre, str) ==> !(isPrefixPred(pre, str))
-{}
-*/
 
 // Sanity check: Dafny should be able to automatically prove the following lemma
 lemma PrefixNegationLemma(pre:string, str:string)
-	ensures  isPrefixPred(pre,str) <==> !isNotPrefixPred(pre,str)	// is a prefix applies both ways
-	ensures !isPrefixPred(pre,str) <==>  isNotPrefixPred(pre,str) // is not a prefix applies both ways
+	ensures  isPrefixPred(pre,str) <==> !isNotPrefixPred(pre,str)
+	ensures !isPrefixPred(pre,str) <==>  isNotPrefixPred(pre,str)
 {}
 
 
 
-
-
-
-
-
-
-
-
-
-// Excplicit char by char checking in the substrings
-predicate isSubstringPred(sub:string, str:string)
-{
-	|str| >= |sub| && exists k :: (0 <= k <= (|str| - |sub|) 
-		==> (forall x :: k <= x < k+|sub| ==> str[x] == sub[x-k]))
-
+predicate isSubstringPred(sub:string, str:string) {
+	|sub| <= |str| && |sub| > 0 &&
+	exists x :: 0 <= x <= (|str| - |sub|) && isPrefixPred(sub, str[x..])
 }
 
-// Using prefix predicate
-predicate isSubstringPred2(sub:string, str:string) {
-	|str| >= |sub| && exists k :: (0 <= k <= (|str| - |sub|) 
-		==> isPrefixPred(sub, str[k..]))
+predicate isNotSubstringPred(sub:string, str:string) {
+	|sub| > |str| || |sub| <= 0 || 
+	forall x :: 0 <= x <= (|str| - |sub|) ==> isNotPrefixPred(sub, str[x..])
 }
 
-// Using sublists
-predicate isSubstringPred3(sub:string, str:string) {
-	|str| >= |sub| && exists k :: (0 <= k <= (|str| - |sub|) 
-		==> str[k..][..|sub|] == sub)
-}
-
-lemma substringPredsAggreee(sub:string, str:string) 
-	//ensures isSubstringPred(sub, str) <==> isSubstringPred2(sub, str) 
-	//ensures isSubstringPred2(sub, str) <==> isSubstringPred3(sub, str) 
-	//ensures isSubstringPred(sub, str) ==> isSubstringPred3(sub, str)
-	//ensures isSubstringPred3(sub, str) ==> isSubstringPred(sub, str) 
-{}
-
-
-predicate isNotSubstringPred(sub:string, str:string)
-{
-	|sub| > |str| && !isSubstringPred(sub, str)
-}
-
-predicate isNotSubstringPred3(sub:string, str:string)
-{
-	|str| < |sub| || !(exists k :: (0 <= k <= (|str| - |sub|) 
-		==> str[k..][..|sub|] == sub))
-}
-
-
-lemma SubstringNegationLemmaExpanded(sub:string, str:string) 
-	ensures isSubstringPred(sub,str) ==> !isNotSubstringPred(sub,str)		// is substring, but not not a substring
-	ensures !isNotSubstringPred(sub,str) ==> isSubstringPred(sub,str)
-	ensures !isSubstringPred(sub,str) ==>  isNotSubstringPred(sub,str)
-	ensures isNotSubstringPred(sub,str) ==> !isSubstringPred(sub,str)
-{}
-
-// Sanity check: Dafny should be able to automatically prove the following lemma
 lemma SubstringNegationLemma(sub:string, str:string)
 	ensures  isSubstringPred(sub,str) <==> !isNotSubstringPred(sub,str)
 	ensures !isSubstringPred(sub,str) <==>  isNotSubstringPred(sub,str)
 {}
 
-lemma SubstringNegationLemmaExpanded3(sub:string, str:string) 
-	ensures isSubstringPred3(sub,str) ==> !isNotSubstringPred3(sub,str)		// is substring, but not not a substring
-	ensures !isNotSubstringPred3(sub,str) ==> isSubstringPred3(sub,str)
-	ensures !isSubstringPred3(sub,str) ==>  isNotSubstringPred3(sub,str)
-	ensures isNotSubstringPred3(sub,str) ==> !isSubstringPred3(sub,str)
-{}
 
 
-
-
-
-
-
-
-
-
-
-
-
-
-
-
-/*
-predicate haveCommonKSubstringPred(k:nat, str1:string, str2:string)
-{
-  //TODO
+predicate haveCommonKSubstringPred(k:nat, str1:string, str2:string) {
+	|str1| >= k && |str2| >= k && 
+	exists x :: 0 <= x <= (|str1| - k) && isSubstringPred(str1[x..][..k], str2) 
 }
 
-predicate haveNotCommonKSubstringPred(k:nat, str1:string, str2:string)
-{
-	//TODO: your FOL formula should start with a forall
+predicate haveNotCommonKSubstringPred(k:nat, str1:string, str2:string) {
+	|str1| < k || |str2| < k ||
+	forall x :: 0 <= x <= (|str1| - k) ==> isNotSubstringPred(str1[x..][..k], str2)
 }
 
 // Sanity check: Dafny should be able to automatically prove the following lemma
@@ -129,4 +59,3 @@ lemma commonKSubstringLemma(k:nat, str1:string, str2:string)
 	ensures  haveCommonKSubstringPred(k,str1,str2) <==> !haveNotCommonKSubstringPred(k,str1,str2)
 	ensures !haveCommonKSubstringPred(k,str1,str2) <==> haveNotCommonKSubstringPred(k,str1,str2)
 {}
-*/
